Merge

ucontrib/CoreCrypto/fst/CoreCrypto.fst
@@ -69,6 +69,8 @@ type dh_key = {
   dh_private : option bytes;
 }
 
+(* TODO: revisit the Tot annotations, switch to EXT when appropriate *)
+
 assume val hash : alg:hash_alg -> bytes -> Tot (h:bytes{length h = hashSize alg})
 assume val hmac : alg:hash_alg -> bytes -> bytes -> Tot (h:bytes{length h = hashSize alg})
 
@@ -98,9 +100,10 @@ assume val dsa_gen_key : int -> EXT dsa_key
 assume val dsa_sign : dsa_key -> bytes -> EXT bytes
 assume val dsa_verify : dsa_key -> bytes -> bytes -> Tot bool
 
-assume val dh_gen_params : int -> dh_params
-assume val dh_gen_key : dh_params -> dh_key
-assume val dh_agreement : dh_key -> bytes -> bytes
+assume val dh_gen_params : int -> EXT dh_params
+assume val dh_gen_key : p:dh_params
+  -> Tot (k:dh_key{k.dh_params = p /\ length k.dh_public <= length p.dh_p})
+assume val dh_agreement : dh_key -> bytes -> Tot bytes
 
 (* type ec_prime = { ecp_prime : string; ecp_order : string; ecp_a : string; ecp_b : string; ecp_gx : string; ecp_gy : string; ecp_bytelen : int; ecp_id : bytes; } *)
 
@@ -108,6 +111,13 @@ type ec_curve =
   | ECC_P256
   | ECC_P384
   | ECC_P521
+
+(* Bytelen of field elements *)
+val ec_bytelen: ec_curve -> Tot int
+let ec_bytelen = function
+  | ECC_P256 -> 32
+  | ECC_P384 -> 48
+  | ECC_P521 -> 66 (* ceil(521/8) *)
 
 type ec_params = {
   curve: ec_curve;
@@ -125,13 +135,15 @@ type ec_key = {
   ec_priv : option bytes;
 }
 
-assume val ec_point_serialize: ec_point -> Tot bytes
 assume val ec_is_on_curve: ec_params -> ec_point -> Tot bool
-assume val ecdh_agreement: ec_key -> ec_point -> bytes
+assume val ecdh_agreement: ec_key -> ec_point -> Tot bytes
 
-assume val ecdsa_sign: option hash_alg -> ec_key -> bytes -> bytes
-assume val ecdsa_verify: option hash_alg -> ec_key -> bytes -> bytes -> bool
-assume val ec_gen_key: ec_params -> ec_key
+assume val ecdsa_sign: option hash_alg -> ec_key -> bytes -> EXT bytes
+assume val ecdsa_verify: option hash_alg -> ec_key -> bytes -> bytes -> Tot bool
+assume val ec_gen_key: p:ec_params
+  -> Tot (k:ec_key{k.ec_params = p /\
+                  length k.ec_point.ecx = ec_bytelen k.ec_params.curve /\
+                  length k.ec_point.ecy = ec_bytelen k.ec_params.curve})
 
 assume val validate_chain: der_list:list bytes -> for_signing:bool -> hostname:option string -> ca_file:string -> Tot bool
 assume val cert_verify_sig: bytes -> sig_alg -> hash_alg -> bytes -> bytes -> Tot bool
